Type classes and theory for IntPow and Abs. CutMinus defined on the total order.

src/interfaces/additional_operations.v
@@ -1,64 +1,68 @@
 Require Import 
   Program Morphisms abstract_algebra.
 
+Class Abs A `{Equiv A} `{Order A} `{RingZero A} `{GroupInv A} 
+  := abs_sig: ∀ (x : A), { y : A | (0 ≤ x → y = x) ∧ (x ≤ 0 → y = -x)}.
+Definition abs `{Abs A} := λ x : A, ` (abs_sig x).
+Instance: Params (@abs_sig) 6.
+Instance: Params (@abs) 6.
+
 Class Pow A B := pow: A → B → A.
 Infix "^" := pow.
 Notation "(^)" := pow (only parsing).
 Instance: Params (@pow) 3.
 
-Inductive nat_pow_spec `{Equiv A} `{Equiv B} `{RingOne A} `{RingMult A} `{RingZero B} 
-    `{RingOne B} `{RingPlus B} : A → B → A → Prop := 
-| nat_pow_spec_0 : `(nat_pow_spec x 0 1)
-| nat_pow_spec_S : `(nat_pow_spec x n y → nat_pow_spec x (1 + n) (x * y))
-| nat_pow_spec_proper': `(x1 = x2 → n1 = n2 → y1 = y2 → 
-    nat_pow_spec x1 n1 y1 → nat_pow_spec x2 n2 y2). 
+Inductive nat_pow_spec `{Equiv A} `{Equiv B} `{RingOne A} `{RingMult A} `{RingZero B} `{RingOne B} `{RingPlus B}  : A → B → A → Prop := 
+  | nat_pow_spec_0 : `(nat_pow_spec x 0 1)
+  | nat_pow_spec_S : `(nat_pow_spec x n y → nat_pow_spec x (1 + n) (x * y))
+  | nat_pow_spec_proper': `(x1 = x2 → n1 = n2 → y1 = y2 → nat_pow_spec x1 n1 y1 → nat_pow_spec x2 n2 y2). 
 
-Class NatPow A B `{Equiv A} `{Equiv B} `{RingOne A} `{RingMult A} `{RingZero B} 
-    `{RingOne B} `{RingPlus B} := nat_pow_sig (x : A) (n : B) : { y | nat_pow_spec x n y }.
-Instance nat_pow `{NatPow A B} : `{Pow A B} := λ x n, ` (nat_pow_sig x n).
+Class NatPow A B `{Equiv A} `{Equiv B} `{RingOne A} `{RingMult A} `{RingZero B} `{RingOne B} `{RingPlus B} 
+  := nat_pow_sig (x : A) (n : B) : { y : A | nat_pow_spec x n y }.
+Instance nat_pow `{NatPow A B} : Pow A B := λ x n, ` (nat_pow_sig x n).
 Instance: Params (@nat_pow_sig) 10.
 Instance: Params (@nat_pow) 10.
 
-(*
-(* [0 ^ x] for a negative [x] is not defined. However, we take the easy way and let it yield [0]. *)
-Class IntPow A B `{OrdField A} `{!DecMultInv A} `{Integers B} := 
-  int_pow_sig (x : A) (n : B) : { y | (0 ≤ n → nat_pow_spec x n y) ∧ (n < 0 → nat_pow_spec x (-n) (/ y)) }.
-Instance int_pow `{IntPow A B} : `{Pow A B} := λ x n, ` (int_pow_sig x n).
-*)
+(* [0 ^ x] is undefined in case [x] is negative. However, we take the easy way, and let it yield [0]. *)
+Class IntPow A B `{Equiv A} `{Equiv B} `{Order B} `{RingOne A} `{RingMult A} `{DecMultInv A} 
+    `{RingZero B} `{RingOne B} `{RingPlus B} `{GroupInv B} 
+  := int_pow_sig: ∀ (x : A) (n : B), { y : A | (0 ≤ n → nat_pow_spec x n y) ∧ (n ≤ 0 → nat_pow_spec x (-n) (/ y)) }.
+Instance int_pow `{IntPow A B} : Pow A B := λ x n, ` (int_pow_sig x n).
+Instance: Params (@int_pow_sig) 17.
+Instance: Params (@int_pow) 17.
 
-Class ShiftLeft A B `{NatPow A B} `{RingPlus A} := shiftl_sig: ∀ (x : A) (y : B), 
-  { z: A | z = x * 2 ^ y }.
+Class ShiftLeft A B `{NatPow A B} `{RingPlus A} 
+  := shiftl_sig: ∀ (x : A) (y : B), { z : A | z = x * 2 ^ y }.
 Definition shiftl `{ShiftLeft A B}: A → B → A := λ x y, ` (shiftl_sig x y).
 Infix "≪" := shiftl (at level 33, left associativity).
 Notation "(≪)" := shiftl (only parsing).
 Instance: Params (@shiftl_sig) 12.
 Instance: Params (@shiftl) 12.
 
-Class Log `(b : A) B  `{NatPow A B} `{RingZero A} `{RingPlus A} `{Order A} :=
-  log_sig: ∀ (x : {z : A | 0 < z }), { z: B | b ^ z ≤ `x < b ^ (z + 1) }.
+Class Log `(b : A) B  `{NatPow A B} `{RingZero A} `{RingPlus A} `{Order A} 
+  := log_sig: ∀ (x : {z : A | 0 < z }), { z : B | b ^ z ≤ `x < b ^ (z + 1) }.
 Definition log  `(b : A) `{Log A b N}: {z | 0 < z } → N := λ x, ` (log_sig x).
 Instance: Params (@log_sig) 15.
 Instance: Params (@log) 15.
 
-(* Our abs operation is of type [Z → N] and therefore quite annoying for this definition *)
-Class Euclid `{Equiv A} `{RingZero A} `{RingPlus A} `{RingMult A} `{Order A} a (b : { z : A | z ≠ 0}) q r := 
-  euclid : a = `b * q + r ∧ (0 ≤ r < `b ∨ `b < r ≤ 0).
+Definition Euclid `{Equiv A} `{Order A} `{RingZero A} `{RingPlus A} `{RingMult A} `{GroupInv A} `{!Abs A} 
+  a (b : { z : A | z ≠ 0}) q r := a = `b * q + r ∧ (0 ≤ r < `b ∨ `b < r ≤ 0).
 
-Class DivEuclid A `{Equiv A} `{RingZero A} `{RingPlus A} `{RingMult A} `{Order A} := div_euclid_sig (a : A) (b : { z : A | z ≠ 0}) : 
-  { q : A | ∃ r, Euclid a b q r }.
-Class ModEuclid A `{Equiv A} `{RingZero A} `{RingPlus A} `{RingMult A} `{Order A} := mod_euclid_sig (a : A) (b : { z : A | z ≠ 0}) : 
-  { r : A | ∃ q, Euclid a b q r }.
+Class DivEuclid A `{Equiv A} `{Order A} `{RingZero A} `{RingPlus A} `{RingMult A} `{GroupInv A} `{!Abs A} 
+  := div_euclid_sig (a : A) (b : { z : A | z ≠ 0}) : { q : A | ∃ r, Euclid a b q r }.
+Class ModEuclid A `{Equiv A} `{Order A} `{RingZero A} `{RingPlus A} `{RingMult A} `{GroupInv A} `{!Abs A} 
+  := mod_euclid_sig (a : A) (b : { z : A | z ≠ 0}) : { r : A | ∃ q, Euclid a b q r }.
 
-Definition div_euclid `{DivEuclid A}: A → { z : A | z ≠ 0} → A := λ x y, ` (div_euclid_sig x y).
-Instance: Params (@div_euclid_sig) 7.
-Instance: Params (@div_euclid) 7.
+Definition div_euclid `{DivEuclid A} : A → { z : A | z ≠ 0} → A := λ x y, ` (div_euclid_sig x y).
+Instance: Params (@div_euclid_sig) 9.
+Instance: Params (@div_euclid) 9.
 
-Definition mod_euclid `{ModEuclid A}: A → { z : A | z ≠ 0} → A := λ x y, ` (mod_euclid_sig x y).
-Instance: Params (@mod_euclid_sig) 7.
-Instance: Params (@mod_euclid) 7.
+Definition mod_euclid `{ModEuclid A} : A → { z : A | z ≠ 0} → A := λ x y, ` (mod_euclid_sig x y).
+Instance: Params (@mod_euclid_sig) 9.
+Instance: Params (@mod_euclid) 9.
 
 Class ShiftRight A B `{NatPow A B} `{RingPlus A} `{Order A}
-  := shiftr_sig: ∀ (x : A) (y : B), { z: A | x ≤ z * 2 ^ y < 2 * x }.
+  := shiftr_sig: ∀ (x : A) (y : B), { z : A | x ≤ z * 2 ^ y < 2 * x }.
 
 Definition shiftr `{ShiftRight A B}: A → B → A := λ x y, proj1_sig (shiftr_sig x y).
 Infix "≫" := shiftr (at level 33, left associativity).
@@ -66,9 +70,9 @@ Notation "(≫)" := shiftr (only parsing).
 Instance: Params (@shiftr_sig) 13.
 Instance: Params (@shiftr) 13.
 
-Class CutMinus A `{Equiv A} `{RingZero A} `{RingPlus A} `{Order A} := 
-  cut_minus_sig: ∀ (x y : A), { z: A | (y < x → z + y = x) ∧ (x ≤ y → z =0) }.
-Definition cut_minus `{m : CutMinus A} : A → A → A := λ x y, ` (cut_minus_sig x y).
+Class CutMinus A `{Equiv A} `{RingZero A} `{RingPlus A} `{Order A}
+  := cut_minus_sig: ∀ (x y : A), { z : A | (y ≤ x → z + y = x) ∧ (x ≤ y → z =0) }.
+Definition cut_minus `{CutMinus A} : A → A → A := λ x y, ` (cut_minus_sig x y).
 Infix "∸" := cut_minus (at level 50, left associativity).
 Notation "(∸)" := cut_minus (only parsing).
 Instance: Params (@cut_minus_sig) 6.
