src/orders/minmax.v
@@ -4,48 +4,48 @@ Require Import
 
 (* This is ugly, maybe we should let TotalOrder live in Type to get rid of the Decision stuff *)
 Section contents.
-  Context `{Setoid A} `{Order A} `{∀ x y: A, Decision (x ≤ y)}.
+  Context `{Setoid A} `{Order A} `{prec_decide : ∀ x y: A, Decision (x ≤ y)}.
 
-  Definition sort (x y: A) : prod A A := if decide (x ≤ y) then (x, y) else (y, x).
+  Definition sort (x y: A) : A * A := if prec_decide x y then (x, y) else (y, x).
 
   Definition min (x y: A) := fst (sort x y).
   Definition max (x y: A) := snd (sort x y).
 
   Lemma min_lb_l x y `{!Reflexive (≤)} `{!TotalOrder (≤)} : min x y ≤ x.
-  Proof. unfold min, sort. case (decide _); firstorder. Qed.
+  Proof. unfold min, sort. case (prec_decide _); firstorder. Qed.
 
   Lemma min_lb_r `{!Reflexive (≤)} x y : min x y ≤ y.
-  Proof. unfold min, sort. case (decide _); firstorder. Qed.
+  Proof. unfold min, sort. case (prec_decide _); firstorder. Qed.
 
   Lemma min_l x y : x ≤ y → min x y = x.
-  Proof. unfold min, sort. case (decide _); firstorder. Qed.
+  Proof. unfold min, sort. case (prec_decide _); firstorder. Qed.
 
   Lemma min_r `{!AntiSymmetric (≤)} x y : y ≤ x → min x y = y.
-  Proof. unfold min, sort. case (decide _); firstorder. Qed.
+  Proof. unfold min, sort. case (prec_decide _); firstorder. Qed.
 
   Lemma min_diag x: min x x = x.
-  Proof. unfold min, sort. case (decide _); reflexivity. Qed.
+  Proof. unfold min, sort. case (prec_decide _); reflexivity. Qed.
 
   Lemma max_ub_l `{!Reflexive (≤)} x y : x ≤ max x y.
-  Proof. unfold max, sort. case (decide _); auto. Qed.
+  Proof. unfold max, sort. case (prec_decide _); auto. Qed.
 
   Lemma max_ub_r `{!Reflexive (≤)} `{!TotalOrder (≤)} x y : y ≤ max x y.
-  Proof. unfold max, sort. case (decide _); firstorder. Qed.
+  Proof. unfold max, sort. case (prec_decide _); firstorder. Qed.
 
   Lemma max_l `{!AntiSymmetric (≤)} x y : y ≤ x → max x y = x.
-  Proof. unfold max, sort. case (decide _); firstorder. Qed.
+  Proof. unfold max, sort. case (prec_decide _); firstorder. Qed.
 
   Lemma max_r x y : x ≤ y → max x y = y.
-  Proof. unfold max, sort. case (decide _); firstorder. Qed.
+  Proof. unfold max, sort. case (prec_decide _); firstorder. Qed.
 
   Lemma max_diag x: max x x = x.
-  Proof. unfold max, sort. case (decide _); reflexivity. Qed.
+  Proof. unfold max, sort. case (prec_decide _); reflexivity. Qed.
   
   Global Instance sort_proper `{!Proper ((=) ==> (=) ==> iff) (≤)} : Proper ((=) ==> (=) ==> (=)) sort.
   Proof with assumption.
     intros x y E x' y' E'.
     unfold sort.
-    do 2 case (decide _); simpl.
+    do 2 case (prec_decide _); simpl.
         firstorder. 
        intros F ?. destruct F. rewrite <-E, <-E'...
       intros ? F. destruct F. rewrite E, E'...
@@ -59,16 +59,16 @@ Section contents.
   Proof. unfold max. repeat intro. apply sm_proper. apply sort_proper; assumption. Qed.
 
   Global Instance min_commutative `{!AntiSymmetric (≤)} `{!TotalOrder (≤)} : Commutative min.
-  Proof. intros x y. unfold min, sort. do 2 case (decide _); firstorder. Qed.
+  Proof. intros x y. unfold min, sort. do 2 case (prec_decide _); firstorder. Qed.
 
   Global Instance max_commutative `{!AntiSymmetric (≤)} `{!TotalOrder (≤)} : Commutative max.
-  Proof. intros x y. unfold max, sort. do 2 case (decide _); firstorder. Qed.
+  Proof. intros x y. unfold max, sort. do 2 case (prec_decide _); firstorder. Qed.
 
   Global Instance min_associative `{!AntiSymmetric (≤)} `{!Transitive (≤)} `{!TotalOrder (≤)} : Associative min.
   Proof with auto; try reflexivity; try contradiction.
      intros x y z. unfold min, sort.
-     case (decide (y ≤ z)); simpl; intros E1; case (decide (x ≤ y)); simpl; intros E2; 
-       case (decide (x ≤ z)); simpl; intros E3; case (decide (y ≤ z)); simpl; intros E4...
+     case (prec_decide y z); simpl; intros E1; case (prec_decide x y); simpl; intros E2; 
+       case (prec_decide x z); simpl; intros E3; case (prec_decide y z); simpl; intros E4...
      destruct E3. transitivity y...
      destruct E4. transitivity x... apply orders.precedes_flip... 
   Qed.
@@ -76,8 +76,8 @@ Section contents.
   Global Instance max_associative `{!AntiSymmetric (≤)} `{!Transitive (≤)} `{!TotalOrder (≤)} : Associative max.
   Proof with auto; try reflexivity; try contradiction.
      intros x y z. unfold max, sort.
-     case (decide (y ≤ z)); simpl; intros E1; case (decide (x ≤ y)); simpl; intros E2; 
-       case (decide (x ≤ z)); simpl; intros E3; case (decide (y ≤ z)); simpl; intros E4...
+     case (prec_decide y z); simpl; intros E1; case (prec_decide x y); simpl; intros E2; 
+       case (prec_decide x z); simpl; intros E3; case (prec_decide y z); simpl; intros E4...
      destruct E3. transitivity y...
      destruct E4. transitivity x... apply orders.precedes_flip... 
   Qed.
@@ -90,7 +90,7 @@ Instance: Params (@max) 3.
 Section order_preserving.
   Context `{PartialOrder A} `{PartialOrder B} {f : A → B} `{!OrderPreserving f}
     `{!TotalOrder (precedes (A:=A))} `{!TotalOrder (precedes (A:=B))}
-    `{∀ x y: A, Decision (x ≤ y)} `{∀ x y: B, Decision (x ≤ y)}. 
+    `{prec_decideA : ∀ x y: A, Decision (x ≤ y)} `{prec_decideB : ∀ x y: B, Decision (x ≤ y)}. 
 
   Instance: Setoid A. apply poset_setoid. Qed.
   Instance: Setoid B. apply poset_setoid. Qed.
@@ -98,7 +98,7 @@ Section order_preserving.
   Lemma preserves_min x y : f (min x y) = min (f x) (f y).
   Proof with auto.
     symmetry. unfold min at 2. unfold sort.
-    case (decide _); simpl; intros E.
+    case (prec_decideA _); simpl; intros E.
      apply min_l. apply (order_preserving _)...
     apply min_r. apply (order_preserving _). apply precedes_flip...
   Qed.
@@ -106,7 +106,7 @@ Section order_preserving.
   Lemma preserves_max x y : f (max x y) = max (f x) (f y).
   Proof with auto.
     symmetry. unfold max at 2. unfold sort.
-    case (decide _); simpl; intros E.
+    case (prec_decideA _); simpl; intros E.
      apply max_r. apply (order_preserving _)...
     apply max_l. apply (order_preserving _). apply precedes_flip...
   Qed.
