src/theory/int_pow.v
@@ -1,153 +1,258 @@
-(* Require
-  theory.naturals orders.semiring theory.integers theory.fields.
+Require
+  theory.naturals orders.semirings orders.integers orders.fields.
 Require Import 
   Program Morphisms Setoid Ring
   abstract_algebra interfaces.naturals interfaces.integers interfaces.additional_operations
-  theory.nat_pow.
+  theory.nat_pow theory.int_abs.
 
 (* * Properties of Int Pow *)
 Section int_pow_properties.
-  Context `{Field A} 
-    `{!LeftCancellation (=) (λ x, x ≠ 0) ring_mult}
-    `{∀ x y, Decision (x = y)}
-    `{Integers B}
-    `{!RingMinus B}.
+Context `{Field A} 
+  `{∀ z, NeZero z → LeftCancellation ring_mult z}
+  `{∀ x y, Decision (x = y)} `{!DecMultInv A}
+  `{Integers B} `{oB : Order B} `{!RingOrder oB} `{!TotalOrder oB}.
 
-  Add Ring A: (rings.stdlib_semiring_theory A).
-  Add Ring B: (rings.stdlib_ring_theory B).
+Add Ring A : (rings.stdlib_semiring_theory A).
+Add Ring B : (rings.stdlib_ring_theory B).
 
-  Context `{ip : !IntPow A B}.
-  Global Instance: Proper ((=) ==> (=) ==> (=)) (^).
-  Proof with eauto.
-    intros x1 y1 E1 x2 y2 E2. 
-    unfold pow, int_pow, int_pow_sig. 
-    destruct ip as [z1 [F1 G1]], ip as [z2 [F2 G2]]. simpl.
-    destruct (orders.precedes_or_precedes_neq 0 x2).
-     eapply nat_pow_spec_unique...
-     eapply nat_pow_spec_proper... reflexivity. 
-     apply F2. rewrite <-E2...
-    apply fields.dec_mult_inv_inj.
-    eapply nat_pow_spec_unique...
-    eapply nat_pow_spec_proper... apply inv_proper... 
-    reflexivity.
-    apply G2. rewrite <-E2...
+Section int_pow_spec_from_properties.
+  Context (f : A → B → A) {f_proper : Proper ((=) ==> (=) ==> (=)) f}
+    ( f_0 : ∀x, f x 0 = 1 ) ( f_S : ∀ x n, 0 ≤ n → f x (1+n) = x * (f x n) ).
+
+  Lemma int_pow_spec_from_properties_nonneg x n : 0 ≤ n → nat_pow_spec x n (f x n).
+  Proof with auto; try reflexivity.
+    intros E. pattern n. apply integers.induction_nonneg...
+      intros a b F. 
+      eapply nat_pow_spec_proper...
+      rewrite F...
+     eapply nat_pow_spec_proper... apply nat_pow_spec_0...
+    intros. eapply nat_pow_spec_proper...
+    eapply nat_pow_spec_S...
   Qed.
 
-  Lemma int_pow_0 x : x ^ (0:B) = 1.
-  Proof with eauto.
-    unfold pow, int_pow, int_pow_sig. destruct ip as [z [Fz Gz]]. simpl.
-    eapply nat_pow_spec_unique. 
-    apply Fz. reflexivity.
-    apply nat_pow_spec_0.
+  Context ( f_inv : ∀ x n,  f x (-n) = /(f x n) ).
+  Lemma int_pow_spec_from_properties x n : 
+    (0 ≤ n → nat_pow_spec x n (f x n)) ∧ (n ≤ 0 → nat_pow_spec x (-n) (/ (f x n))).
+  Proof with trivial.
+    split.
+     apply int_pow_spec_from_properties_nonneg.
+    intros. eapply (nat_pow_spec_proper _ _ (reflexivity _) _ _ (reflexivity _)).
+     symmetry...
+    apply int_pow_spec_from_properties_nonneg.
+    apply rings.flip_nonpos_inv...
   Qed.
+End int_pow_spec_from_properties.
 
-  Lemma int_pow_S_pos (x : A) (n : B) : 0 ≤ n → x ^ (1+n) = x * x ^ n.
-  Proof with eauto.
-    intros E.
-    unfold pow, int_pow, int_pow_sig. 
-    destruct ip as [z1 [F1 G1]], ip as [z2 [F2 G2]]. simpl.
-    eapply nat_pow_spec_unique. 
-    apply F1. apply semiring.sr_precedes_nonneg_plus_compat...
-     apply semiring.sr_precedes_0_1...
-    apply nat_pow_spec_S...
-  Qed.
-  
-  Lemma int_pow_S_neg (x : A) (n : B) : x ≠ 0 → n < 0 → x ^ (1+n) = x * x ^ n.
-  Proof with eauto.
-    intros E1 E2.
-    unfold pow, int_pow, int_pow_sig. 
-    destruct ip as [z1 [F1 G1]], ip as [z2 [F2 G2]]. simpl.
-    apply fields.dec_mult_inv_inj.
-    eapply nat_pow_spec_unique.
-     apply G1. admit.
-    assert (-(1 + n) = 1 + -(1) + -(n + 1)) as E2 by ring. (* rewrite hangs... *)
-    eapply nat_pow_spec_proper.  reflexivity. apply E2.
-     rewrite fields.dec_mult_inv_distr, fields.dec_mult_inv_involutive. reflexivity.
-    apply nat_pow_spec_S.
-    apply G2.
-    admit.
-  Qed.
+Context `{ip : !IntPow A B}.
+Global Instance: Proper ((=) ==> (=) ==> (=)) (^).
+Proof with eauto.
+  intros x y E1 n m E2. 
+  unfold pow, int_pow, int_pow_sig. 
+  destruct ip as [z1 [Ez1 Fz1]], ip as [z2 [Ez2 Fz2]]. simpl.
+  destruct (total_order 0 n).
+   eapply nat_pow_spec_unique...
+   eapply nat_pow_spec_proper... reflexivity.
+   apply Ez2. rewrite <-E2...
+  apply fields.dec_mult_inv_inj.
+  eapply nat_pow_spec_unique...
+  eapply nat_pow_spec_proper... apply inv_proper... 
+  reflexivity.
+  apply Fz2. rewrite <-E2...
+Qed.
 
-  Instance: RightIdentity (^) (1:B).
-  Proof. 
-    intro. assert ((1:B) = 1 + 0) as E by ring. rewrite E.
-    rewrite int_pow_S_pos, int_pow_0. ring.
-    reflexivity.
-  Qed.
+Lemma int_pow_0 x : x ^ (0:B) = 1.
+Proof with eauto.
+  unfold pow, int_pow, int_pow_sig. destruct ip as [z [Fz Gz]]. simpl.
+  eapply nat_pow_spec_unique. 
+  apply Fz. reflexivity.
+  apply nat_pow_spec_0.
+Qed.
 
-  Instance: LeftAbsorb (pow (B:=B)) (1 : A).
-  Proof with auto. 
-    intro. 
-    pattern y. apply integers.induction; clear y.
-       intros ? ? E. rewrite E. tauto.
-      apply int_pow_0.
-     intros n E F.
-     rewrite int_pow_S_pos... rewrite F. ring.
-    intros n E F. admit. (*rewrite int_pow_S_neg in F... ring_simplify in F... *)
-  Qed.
+Lemma int_pow_mult_inv (x : A) (n : B) : x ^(-n) = /(x ^ n).
+Proof with auto.
+  unfold pow, int_pow, int_pow_sig. 
+  destruct (ip x n) as [z2 [Ez2 Fz2]]. destruct ip as [z1 [Ez1 Fz1]]. simpl.
+  destruct (total_order 0 n).
+   apply fields.dec_mult_inv_inj.
+   eapply nat_pow_spec_unique.
+    apply Fz1, rings.flip_nonneg_inv...
+   eapply (nat_pow_spec_proper _ _ (reflexivity _)).
+     apply rings.inv_involutive.
+    apply fields.dec_mult_inv_involutive.
+   apply Ez2...
+  eapply nat_pow_spec_unique.
+   apply Ez1, rings.flip_nonpos_inv...
+  apply Fz2...
+Qed.
 
-  Lemma int_pow_zero (x: B) : x ≠ 0 → 0 ^ x = 0.
-  Proof with eauto.
-    pattern x. apply integers.induction; clear x.
-       intros ? ? E. rewrite E. tauto.
-      intro E. destruct E. reflexivity.
-     intros x E F G. rewrite int_pow_S_pos... ring.
-    intros x E F G. admit. (* rewrite <-rings.mult_1_l. rewrite <-int_pow_S_neg... ring. *)
-  Qed. 
+Lemma int_pow_mult_inv_alt (x : A) (n : B) : x ^n = /(x ^ (-n)).
+Proof.
+  rewrite <-int_pow_mult_inv.
+  rewrite rings.inv_involutive.
+  reflexivity.
+Qed.
 
-  Lemma int_pow_exp_sum (x y: B) (n: A) : 
-    n ^ (x + y) = n ^ x * n ^ y.
+Lemma int_pow_S_nonneg (x : A) (n : B) : 0 ≤ n → x ^ (1+n) = x * x ^ n.
+Proof with eauto.
+  intros E.
+  unfold pow, int_pow, int_pow_sig. 
+  destruct ip as [z1 [F1 G1]], ip as [z2 [F2 G2]]. simpl.
+  eapply nat_pow_spec_unique. 
+  apply F1. apply semirings.nonneg_plus_compat...
+   apply semirings.precedes_0_1...
+  apply nat_pow_spec_S...
+Qed.
+
+Lemma int_pow_S (x : A) (n : B) : x ≠ 0 →  x ^ (1+n) = x * x ^ n.
+Proof with auto.
+  intros E.
+  destruct (orders.precedes_or_sprecedes 0 n).
+   apply int_pow_S_nonneg...
+   rewrite int_pow_mult_inv_alt, (int_pow_mult_inv_alt _ n).
+  setoid_replace (-n) with (1 - (1 + n)) by ring.
+  rewrite int_pow_S_nonneg.
+  rewrite fields.dec_mult_inv_distr. rewrite associativity. 
+  rewrite fields.dec_mult_inverse... ring.
+  apply rings.flip_nonpos_inv...
+  rewrite commutativity.
+  apply integers.precedes_sprecedes_alt...
+Qed.
+
+Lemma int_pow_nat_pow `{Naturals N} `{!NatPow A N} (x : A) (n : N) :
+  x ^ (naturals_to_semiring N B n) = x ^ n.
+Proof.
+  revert n. apply naturals.induction.
+    intros ? ? E. rewrite E. reflexivity.
+   rewrite rings.preserves_0, int_pow_0, nat_pow_0. reflexivity.
+  intros n E.
+  rewrite rings.preserves_plus, rings.preserves_1.
+  rewrite int_pow_S_nonneg, nat_pow_S.
+   rewrite E. reflexivity.
+  apply naturals.to_semiring_nonneg.
+Qed.
+
+Instance: RightIdentity (^) (1:B).
+Proof. 
+  intro. assert ((1:B) = 1 + 0) as E by ring. rewrite E.
+  rewrite int_pow_S_nonneg, int_pow_0. ring.
+  reflexivity.
+Qed.
+
+Instance: LeftAbsorb (pow (B:=B)) (1 : A).
+Proof with auto. 
+  intro n. 
+  pattern n. apply integers.induction; clear n.
+     intros ? ? E. rewrite E. tauto.
+    apply int_pow_0.
+   intros n E F.
+   rewrite int_pow_S_nonneg... rewrite F. ring.
+  intros n E F. 
+  setoid_replace n with (1 + (n - 1)) in F by ring.
+  rewrite int_pow_S in F. ring_simplify in F...
+  apply (ne_zero 1).
+Qed.
+
+Lemma int_pow_exp_sum (n m: B) (x : A) : 
+  x ≠ 0 → x ^ (n + m) = x ^ n * x ^ m.
+Proof with auto.
+  intros nonneg.
+  pattern n. apply integers.induction; clear n.
+     intros ? ? E. rewrite E. tauto.
+    rewrite int_pow_0, left_identity. ring.
+   intros ? ? E. 
+   rewrite <-associativity.
+   rewrite int_pow_S... rewrite E. rewrite int_pow_S... ring.
+  intros ? ? E.
+  apply (rings.left_cancellation_ne_0 ring_mult x)... rewrite associativity.
+  rewrite <-int_pow_S... rewrite <-int_pow_S...
+  setoid_replace (1 + (n - 1 + m)) with (n + m) by ring.
+  setoid_replace (1 + (n - 1)) with n by ring...
+Qed.
+
+Lemma int_pow_of_0 (n : B) : n ≠ 0 → 0 ^ n = 0.
+Proof with auto.
+  pattern n. apply integers.induction; clear n.
+     intros ? ? E. rewrite E. tauto.
+    intro E. destruct E. reflexivity.
+   intros. rewrite int_pow_S_nonneg... ring.
+  intros n ? ? ?. rewrite int_pow_mult_inv_alt.
+  setoid_replace (-(n - 1)) with (1 - n) by ring.
+  rewrite int_pow_S_nonneg. 
+   rewrite left_absorb. apply fields.dec_mult_inv_0.
+  apply rings.flip_nonpos_inv...
+Qed.
+End int_pow_properties.
+
+Section preservation.
+  Context 
+    `{Integers B} `{oB : Order B} `{!RingOrder oB} `{!TotalOrder oB}
+    `{Field A1} `{∀ z : A1, NeZero z → LeftCancellation ring_mult z} `{∀ x y : A1, Decision (x = y)} `{!DecMultInv A1} `{!IntPow A1 B}
+    `{Field A2} `{∀ z : A2, NeZero z → LeftCancellation ring_mult z} `{∀ x y : A2, Decision (x = y)} `{!DecMultInv A2} `{!IntPow A2 B}
+    {f : A1 → A2} `{!OrderPreserving f} `{!Ring_Morphism f} `{!Injective f}.
+
+  Add Ring B2 : (rings.stdlib_ring_theory B).
+
+  Lemma preserves_int_pow x (n : B) : f (x ^ n) = (f x) ^ n.
   Proof with auto.
-    pattern x. apply integers.induction; clear x.
-      intros ? ? E. rewrite E. tauto.
-     rewrite int_pow_0, left_identity. ring.
-    intros ? ? E. 
-     rewrite <-associativity.
-     rewrite int_pow_S_pos. rewrite int_pow_S_pos. rewrite E. ring.
-    destruct (decide (n = 0)) as [F|F].
-    rewrite <-associativity in E.
-    do 2 rewrite int_pow_S in E. 
-    apply (left_cancellation ring_mult n).
+    revert n. apply integers.induction.
+       intros ? ? E1. rewrite E1. reflexivity.
+      rewrite int_pow_0, int_pow_0. apply rings.preserves_1.
+     intros n E F. 
+     rewrite int_pow_S_nonneg, rings.preserves_mult, F...
+     rewrite int_pow_S_nonneg... reflexivity.
+    intros n E F.
+    destruct (decide (x = 0)) as [G | G].
+     rewrite G. rewrite rings.preserves_0. 
+     assert (n - 1 ≠ 0).
+      apply orders.neq_precedes_sprecedes, integers.precedes_sprecedes_alt.
+      ring_simplify...
+     repeat rewrite int_pow_of_0...
+     apply rings.preserves_0.
+    assert (f x ≠ 0). apply rings.injective_not_0...
+    apply (rings.left_cancellation_ne_0 ring_mult (f x))...
+    rewrite <-int_pow_S, <-rings.preserves_mult, <-int_pow_S...
+    setoid_replace (1 + (n - 1)) with n by ring...
   Qed.
-  
-  Context `{!NoZeroDivisors A} `{!ZeroNeOne A}.
-
-  Lemma nat_pow_nonzero (x: B) (n: A) : n ≠ 0 → n ^ x ≠ 0.
-  Proof with eauto.
-    pattern x. apply naturals.induction; clear x.
-    intros x1 x2 E. rewrite E. tauto.
-    intros. rewrite nat_pow_0. apply not_symmetry. apply zero_ne_one.
-    intros x E F G. rewrite nat_pow_S in G.
-    apply (no_zero_divisors n); split... 
-  Qed. 
-End nat_pow_properties.
+End preservation.
 
 (* Very slow default implementation by translation into Peano *)
 Section int_pow_default.
   Context `{Field A} 
-    `{!LeftCancellation (=) (λ x, x ≠ 0) ring_mult}
-    `{∀ x y, Decision (x = y)}
-    `{Integers B}.
-  
-  Fixpoint nat_pow_rec (x: A) (n : nat) : A := match n with
-  | 0 => 1
-  | S n => x * (nat_pow_rec x n)
-  end.
+    `{∀ z, NeZero z → LeftCancellation ring_mult z}
+    `{∀ x y, Decision (x = y)} `{!DecMultInv A}
+    `{Integers B} `{oB : Order B} `{!RingOrder oB} `{!TotalOrder oB}.
 
-  Instance: Proper ((=) ==> (=) ==> (=)) nat_pow_rec.
-  Proof with try reflexivity.
-   intros x y E a ? [].
-   induction a; simpl...
-   rewrite IHa, E...
-  Qed.
+  Let int_pow_default (x : A) (n : B) : A := 
+    match (decide (0 ≤ n)) with
+    | left _ => x ^ (int_abs B nat n)
+    | right _ => /(x ^ (int_abs B nat n))
+    end.
 
-  Let nat_pow_default x n := nat_pow_rec x (naturals_to_semiring B nat n).
-  Global Program Instance: NatPow A B | 10 := nat_pow_default.
-  Next Obligation with simpl; try reflexivity.
-    apply nat_pow_spec_from_properties; unfold nat_pow_default.
-    intros ? ? E ? ? F. rewrite E, F...
-    intros. rewrite rings.preserves_0...
-    intros. rewrite rings.preserves_plus, rings.preserves_1, <-peano_naturals.S_nat_1_plus...
+  Global Program Instance: IntPow A B | 10 := int_pow_default.
+  Next Obligation with try contradiction; auto using semirings.precedes_0_1.
+    apply int_pow_spec_from_properties; unfold int_pow_default.
+       admit.
+      intros y.
+      case (decide _); intros E.
+       rewrite int_abs_0. apply nat_pow_0.
+      destruct E. reflexivity.
+     intros y m E.
+     case (decide _); case (decide _); intros E1 E2...
+      rewrite int_abs_nonneg_plus, int_abs_1...
+      apply nat_pow_S.
+     destruct E2. apply semirings.nonneg_plus_compat_l...
+    intros y m.
+    case (decide _); case (decide _); intros E1 E2...
+       setoid_replace m with (0 : B).
+        rewrite rings.opp_0, int_abs_0, nat_pow_0. symmetry. apply fields.dec_mult_inv_1.
+       apply (antisymmetry (≤))... apply rings.flip_nonpos_inv...
+      rewrite fields.dec_mult_inv_involutive, int_abs_opp. reflexivity.
+     rewrite int_abs_opp. reflexivity.
+    setoid_replace m with (0 : B).
+     rewrite rings.opp_0, int_abs_0, nat_pow_0. rewrite fields.dec_mult_inv_1 at 2. reflexivity.
+    apply (antisymmetry (≤)).
+     apply orders.precedes_flip...
+    apply rings.flip_nonneg_inv.
+    apply orders.precedes_flip...
   Qed.
-End nat_pow_default.
-*)
+End int_pow_default.
